%TCIDATA{Version=5.50.0.2890}
%TCIDATA{LaTeXparent=1,1,pbes-implementation-notes.tex}
                      

\section{PBES rewriters}

In this section we describe two PBES rewriters. We assume that a data
rewriter $r$ is given that rewrites data terms.

\subsection{Simplifying rewriter}

We define a simplifying PBES rewriter $R$ recursively as follows. We assume
that $D$ is a non-empty data type, and we denote the free variables
appearing in $\varphi $ as $\mathsf{free}(\varphi )$. We assume that a data
rewriter $r$ is given that rewrites data terms.%
\begin{equation*}
\begin{array}{lcl}
b & \rightarrow & r(b) \\ 
\lnot \lnot \varphi & \rightarrow & \varphi \\ 
\varphi \wedge true & \rightarrow & \varphi \\ 
true\wedge \varphi & \rightarrow & \varphi \\ 
\varphi \wedge false & \rightarrow & false \\ 
false\wedge \varphi & \rightarrow & false \\ 
\varphi \wedge \varphi & \rightarrow & \varphi \\ 
\varphi \vee true & \rightarrow & true \\ 
true\vee \varphi & \rightarrow & true \\ 
\varphi \vee false & \rightarrow & \varphi \\ 
false\vee \varphi & \rightarrow & \varphi \\ 
\varphi \vee \varphi & \rightarrow & \varphi \\ 
\varphi \Rightarrow \psi & \rightarrow & \lnot \varphi \vee \psi \\ 
\forall _{d:D}.\varphi & \rightarrow & \varphi \text{ if }d\notin \mathsf{%
free}(\varphi ) \\ 
\forall _{d:D}.\lnot \varphi & \rightarrow & \lnot \exists _{d:D}.\varphi \\ 
\forall _{d:D}.\varphi \wedge \psi & \rightarrow & \forall _{d:D}.\varphi
\wedge \forall _{d:D}.\psi \\ 
\forall _{d:D}.\varphi \vee \psi & \rightarrow & (\forall _{d:D}.\varphi
)\vee \psi \text{ if }d\notin \mathsf{free}(\psi ) \\ 
\forall _{d:D}.\varphi \vee \psi & \rightarrow & \varphi \vee (\forall
_{d:D}.\psi )\text{ if }d\notin \mathsf{free}(\varphi ) \\ 
\exists _{d:D}.\varphi & \rightarrow & \varphi \text{ if }d\notin \mathsf{%
free}(\varphi ) \\ 
\exists _{d:D}.\lnot \varphi & \rightarrow & \lnot \forall _{d:D}.\varphi \\ 
\exists _{d:D}.\varphi \vee \psi & \rightarrow & \exists _{d:D}.\varphi \vee
\exists _{d:D}.\psi \\ 
\exists _{d:D}.\varphi \wedge \psi & \rightarrow & (\exists _{d:D}.\varphi
)\wedge \psi \text{ if }d\notin \mathsf{free}(\psi ) \\ 
\exists _{d:D}.\varphi \wedge \psi & \rightarrow & \varphi \wedge (\exists
_{d:D}.\psi )\text{ if }d\notin \mathsf{free}(\varphi ) \\ 
X(e) & \rightarrow & X(r(e))%
\end{array}%
\end{equation*}%
where $\varphi $ and $\psi $ are arbitrary pbes expressions, $b$ is a data
term of data sort $\mathbb{B}$, $true$ and $false$ are elements of data sort 
$\mathbb{B}$, $X$ is a predicate variable, $e$ consists of zero or more data
sorts and $d$ is a data variable of sort $D$.

\paragraph{\newpage Simplify}

The pbes expression rewrite system \textsc{Simplify} [Luc Engelen, 2007]
consists of the following rules\footnote{%
Todo: reformulate this rewrite system.}:%
\begin{eqnarray*}
false\wedge x &\rightarrow &false \\
x\wedge false &\rightarrow &false \\
true\wedge x &\rightarrow &x \\
x\wedge true &\rightarrow &x \\
\lnot true &\rightarrow &false \\
\lnot false &\rightarrow &true \\
ITE(true,x,y) &\rightarrow &x \\
ITE(false,x,y) &\rightarrow &y \\
x &=&x\rightarrow true \\
y &=&x\rightarrow x=y,\text{ provided }y\succ x
\end{eqnarray*}

\subsection{The predicate formula normal form (PFNF)}

\begin{definition}
A predicate formula is said to be in \emph{Predicate Formula Normal Form}
(PFNF) if it has the following form: 
\begin{equation*}
\mathsf{Q}_{1}v_{1}{:}V_{1}.\cdots \mathsf{Q}_{n}v_{n}{:}V_{n}.~h\wedge
\bigwedge\limits_{i\in I}\left( g_{i}\implies \bigvee\limits_{j\in
J_{i}}~X^{j}(e^{j})\right)
\end{equation*}%
where $X^{j}\in \chi $ ($\chi $ is a countable of sorted predicate
variables), $\mathsf{Q}_{i}\in \{\forall ,\exists \}$, $I$ is a (possibly
empty) finite index set, each $J_{i}$ is a non-empty finite index set, and $%
h $ and every $g_{i}$ are simple formulae.
\end{definition}

Note that here $J_{i}$ is used to index a set of occurrences of not
necessarily different variables. For instance, $(n>0\implies X(3)\vee
X(5)\vee Y(6))$ is a formula complying to the definition of PFNF. So long as
it does not lead to confusion, we stick to the convention to drop the typing
of the quantified variables $v_{i}$. An algorithm to compute a PFNF is:

\begin{equation*}
\begin{array}{lll}
p(c) & =_{def} & c \\ 
p(X(d)) & =_{def} & X(d) \\ 
p(\forall {x{:}D}.\varphi ) & =_{def} & \forall {x{:}D}.p(\varphi ) \\ 
p(\exists {x{:}D}.\varphi ) & =_{def} & \exists {x{:}D}.p(\varphi ) \\ 
&  &  \\ 
p(\varphi \wedge \psi ) & =_{def} & 
\begin{array}{l}
\mathsf{Q}_{1}^{\varphi }\cdots \mathsf{Q}_{n^{\varphi }}^{\varphi }\mathsf{Q%
}_{1}^{\psi }\cdots \mathsf{Q}_{n^{\psi }}^{\psi }.~~\left( h^{\varphi
}\wedge h^{\psi }\right) \\ 
\wedge \bigwedge\limits_{i\in I^{\varphi }\cup I^{\psi }}\left(
g_{i}\implies \bigvee\limits_{j\in J_{i}}~X^{j}(e^{j})\right)%
\end{array}
\\ 
&  &  \\ 
p(\varphi \vee \psi ) & =_{def} & 
\begin{array}{l}
\mathsf{Q}_{1}^{\varphi }\cdots \mathsf{Q}_{n^{\varphi }}^{\varphi }\mathsf{Q%
}_{1}^{\psi }\cdots \mathsf{Q}_{n^{\psi }}^{\psi }.\left( h^{\varphi }\vee
h^{\psi }\right) \\ 
\wedge \bigwedge\limits_{i\in I^{\varphi }}\left( \left( \lnot h^{\psi
}\wedge g_{i}\right) \implies \bigvee\limits_{j\in J_{i}}~X^{j}(e^{j})\right)
\\ 
\wedge \bigwedge\limits_{i\in I^{\psi }}\left( \left( \lnot h^{\varphi
}\wedge g_{i}\right) \implies \bigvee\limits_{j\in J_{i}}~X^{j}(e^{j})\right)
\\ 
\wedge \bigwedge\limits_{i\in I^{\varphi },k\in I^{\psi }}\left( \left(
g_{i}\wedge g_{k}\right) \implies \bigvee\limits_{j\in J_{i},m\in
J_{k}}~X^{j}(e^{j})\vee X^{m}(e^{m})\right)%
\end{array}%
\end{array}%
\end{equation*}%
where

\begin{equation*}
\begin{array}{lll}
p(\varphi ) & = & \mathsf{Q}_{1}^{\varphi }\cdots \mathsf{Q}_{n^{\varphi
}}^{\varphi }.~h^{\varphi }\wedge \bigwedge\limits_{i\in I^{\varphi }}\left(
g_{i}\implies \bigvee\limits_{j\in J_{i}}~X^{j}(e^{j})\right)  \\ 
p(\psi ) & = & \mathsf{Q}_{1}^{\psi }\cdots \mathsf{Q}_{n^{\psi }}^{\psi
}.~h^{\psi }\wedge \bigwedge\limits_{i\in I^{\psi }}\left( g_{i}\implies
\bigvee\limits_{j\in J_{i}}~X^{j}(e^{j})\right) ,%
\end{array}%
\end{equation*}%
under the assumption that $I^{\varphi }$ and $I^{\psi }$ are disjoint, and $%
v_{i}^{\varphi }\neq v_{j}^{\psi }$ for all $i,j$.\newpage 

\subsection{OnePointRule Quantifier Elimination}

\subsubsection{Equalities / inequalities}

The function $Eq$ computes a set of equalities and inequalities for an
expression $\varphi $, such that the following holds:%
\begin{eqnarray*}
Eq\left( \varphi \right) &=&\left( \left\{ b_{1}=e_{1},\cdots
,b_{n}=e_{n}\right\} ,W\right) \Rightarrow \varphi =\psi \wedge
\bigwedge\limits_{i=1}^{n}\left( b_{i}=e_{i}\right) \\
Eq\left( \varphi \right) &=&\left( V,\left\{ b_{1}\neq e_{1},\cdots
,b_{n}\neq e_{n}\right\} ,W\right) \Rightarrow \varphi =\psi \vee
\bigvee\limits_{i=1}^{n}\left( b_{i}\neq e_{i}\right)
\end{eqnarray*}%
for some expression $\psi $.

The function $Eq$ is inductively defined as follows:

\begin{equation*}
\begin{array}{lll}
Eq(b) & = & \left( \left\{ b=true\right\} ,\emptyset \right)  \\ 
Eq(d=e) & = & \left\{ 
\begin{array}{cc}
\left( \left\{ d=e\right\} ,\emptyset \right)  & \text{if }d\notin FV(e) \\ 
\left( \emptyset ,\emptyset \right)  & \text{otherwise}%
\end{array}%
\right.  \\ 
Eq(e=d) & = & Eq(d=e) \\ 
Eq(d\neq e) & = & \left\{ 
\begin{array}{cc}
\left( \emptyset ,\left\{ d\neq e\right\} \right)  & \text{if }d\notin FV(e)
\\ 
\left( \emptyset ,\emptyset \right)  & \text{otherwise}%
\end{array}%
\right.  \\ 
Eq(e\neq d) & = & Eq(d\neq e) \\ 
Eq\left( \lnot \varphi \right)  & = & swap\left( Eq\left( \varphi \right)
\right)  \\ 
Eq\left( \varphi \wedge \psi \right)  & = & join\_and\left( \left( Eq\left(
\varphi \right) ,Eq\left( \psi \right) \right) \right)  \\ 
Eq\left( \varphi \vee \psi \right)  & = & join\_or\left( \left( Eq\left(
\varphi \right) ,Eq\left( \psi \right) \right) \right)  \\ 
Eq\left( \varphi \Rightarrow \psi \right)  & = & join\_or\left( \left(
swap\left( Eq\left( \varphi \right) \right) ,Eq\left( \psi \right) \right)
\right)  \\ 
Eq\left( \forall x.\varphi \right)  & = & delete\left( x,Eq\left( \varphi
\right) \right)  \\ 
Eq\left( \exists x.\varphi \right)  & = & delete\left( x,Eq\left( \varphi
\right) \right)  \\ 
Eq\left( \varphi \right)  & = & \left( \emptyset ,\emptyset \right) \text{
otherwise}%
\end{array}%
\end{equation*}%
where $b$ is a boolean data variable, $d$ is an arbitrary data variable, $e$
is a boolean data expression, and%
\begin{equation*}
\begin{array}{lll}
swap\left( \left( V,W\right) \right)  & = & \left( W,V\right)  \\ 
join\_and\left( \left( V_{1},W_{1}\right) ,\left( V_{2},W_{2}\right) \right) 
& = & \left( V_{1}\cup V_{2},W_{1}\cap W_{2}\right)  \\ 
join\_or\left( \left( V_{1},W_{1}\right) ,\left( V_{2},W_{2}\right) \right) 
& = & \left( V_{1}\cap V_{2},W_{1}\cup W_{2}\right)  \\ 
delete\left( x,\left( V,W\right) \right)  & = & 
\begin{array}{l}
\left( V_{1},W_{1}\right) \text{ where} \\ 
\left\{ 
\begin{array}{c}
V_{1}=\left\{ d=e\in V\mid d\neq x\right\}  \\ 
W_{1}=\left\{ d\neq e\in W\mid d\neq x\right\} 
\end{array}%
\right. 
\end{array}%
\end{array}%
\end{equation*}

\subsubsection{OnePointRule rewriter}

We define the OnePointRule rewriter $R$ inductively as follows:

\begin{equation*}
\begin{array}{lll}
R\left( \lnot \varphi \right)  & = & \lnot R\left( \varphi \right)  \\ 
R\left( \varphi \wedge \psi \right)  & = & R\left( \varphi \right) \wedge
R\left( \psi \right)  \\ 
R\left( \varphi \vee \psi \right)  & = & R\left( \varphi \right) \vee
R\left( \psi \right)  \\ 
R\left( \varphi \Rightarrow \psi \right)  & = & R\left( \varphi \right)
\Rightarrow R\left( \psi \right)  \\ 
R\left( \forall x.\varphi \right)  & = & \left\{ 
\begin{array}{cc}
R\left( \varphi \right) \left[ x:=e\right]  & \text{if }x\neq e\in W\text{,
where }\left( V,W\right) =Eq\left( \varphi \right)  \\ 
\forall x.R\left( \varphi \right)  & \text{otherwise}%
\end{array}%
\right.  \\ 
R\left( \exists x.\varphi \right)  & = & \left\{ 
\begin{array}{cc}
R\left( \varphi \right) \left[ x:=e\right]  & \text{if }x=e\in V\text{,
where }\left( V,W\right) =Eq\left( \varphi \right)  \\ 
\exists x.R\left( \varphi \right)  & \text{otherwise}%
\end{array}%
\right.  \\ 
R\left( \varphi \right)  & = & \varphi \text{ otherwise}%
\end{array}%
\end{equation*}

\newpage 
